WIP: more instances for HO

io/TC.Instrumentable.IIOwp.fst
@@ -46,6 +46,8 @@ let enforce_post
   if post_c.result_check x h r lt then r
   else Inr Contract_failure
 
+(** TODO: add importable/exportable types here **)
+
 instance instrumentable_IIO 
   (#t1:Type) (#t2:Type) {| d1:mlfo t1 |} {| d2:mlfo t2 |}
   (pre : t1 -> trace -> Type0)
@@ -54,7 +56,77 @@ instance instrumentable_IIO
   (pi : monitorable_prop) {| post_c:monitorable_post pre post pi |} : 
   instrumentable ((x:t1) -> IIO (maybe t2) (pre x) (post x)) =
   { inst_type = t1 -> IIOpi (maybe t2) pi;
-    cinst_type = ml_instrumented_iio t1 (maybe t2) #(ML_FO d1) #(ML_FO (mlfo_maybe t2)) pi;
+    cinst_type = ml_instrumented_iio t1 (maybe t2) #(ML_FO d1) #(ML_FO (mlfo_maybe t2 #(ML_FO d2))) pi;
     strengthen = (fun (f:(t1 -> IIOpi (maybe t2) pi)) ->
       enforce_post #t1 #t2 pi pre post #post_c f)
+  }
+
+(** ** Higher order **)
+
+(** 
+Be the following example:
+  type ftype = a -> IO b fpre fpost
+  val prog: (ctx: (f:ftype -> IO c cpre cpost) -> IO d ppre ppost.
+For ctx to be instrumentable, the post of f should also respect pi. 
+The post-condition of the ctx must respect pi, but because f is not instrumented, it can break this guarantee. Therefore, f can be mlifyied if its post implies the pi. **)
+class mlifyable_guarded (a b:Type) pre post pi =
+  { cmlifyable : mlifyable ((x:a) -> IIO b (pre x) (post x));
+    cpi : squash (forall (x:a) h lt r. pre x h /\ post x h r lt ==> enforced_locally pi h lt) }
+
+(** 
+this instance should let us mlify example 1.
+the problems here are the following:
+1. c is a ml type.
+2. enforce_post appears here in a kind of weird position **)
+
+let import_out t1 t2 {| d0:importable (maybe t2) |} (pi:monitorable_prop) 
+  (f:t1 -> IIOpi d0.itype pi) 
+  (x:t1) : 
+  IIOpi (maybe t2) pi =
+  match import (f x) with
+  | Some x' -> x'
+  | None -> Inr Contract_failure
+
+instance instrumentable_HO
+  fin fout fpre fpost 
+  cout cpre cpost 
+  pi 
+  {| d0:importable (maybe cout) |}
+  {| d1:mlifyable_guarded fin fout fpre fpost pi |}
+  {| d2:monitorable_post (fun x -> cpre) (fun x -> cpost) pi |} : 
+  instrumentable ((x:fin -> IIO fout (fpre x) (fpost x)) -> DM.IIO.IIO (maybe cout) cpre cpost) =
+  {
+    inst_type = d1.cmlifyable.matype -> IIOpi d0.itype pi;
+    cinst_type = ml_instrumented_iio d1.cmlifyable.matype d0.itype #(ML_ARROW d1.cmlifyable.cmatype) #(ML_FO d0.citype) pi;
+    strengthen = (fun (ctx:(d1.cmlifyable.matype -> IIOpi d0.itype pi)) -> 
+      (fun (f:(x:fin -> IIO fout (fpre x) (fpost x))) -> 
+        (** TODO: import the result **)
+        (let ctx' = import_out d1.cmlifyable.matype cout #d0 pi ctx in
+        enforce_post pi (fun x -> cpre) (fun x -> cpost) #d2 ctx' (d1.cmlifyable.mlify f)) <: IIO (maybe cout) cpre cpost))
+  }
+
+let strengthen_out t1 t2 {| d0:instrumentable t2 |} (pi:monitorable_prop) 
+  (f:t1 -> IIOpi (maybe d0.inst_type) pi) 
+  (x:t1) : 
+  IIOpi (maybe t2) pi =
+  match (f x) with
+  | Inl g -> Inl (d0.strengthen g)
+  | Inr err -> Inr err
+
+instance instrumentable_HO_2
+  fin fout fpre fpost 
+  cout cpre cpost 
+  pi 
+  {| d0:instrumentable cout |}
+  {| d1:mlifyable_guarded fin fout fpre fpost pi |}
+  {| d2:monitorable_post (fun x -> cpre) (fun x -> cpost) pi |} : 
+  instrumentable ((x:fin -> IIO fout (fpre x) (fpost x)) -> DM.IIO.IIO (maybe cout) cpre cpost) =
+  {
+    inst_type = d1.cmlifyable.matype -> IIOpi (maybe d0.inst_type) pi;
+    cinst_type = ml_instrumented_iio d1.cmlifyable.matype (maybe d0.inst_type) #(ML_ARROW d1.cmlifyable.cmatype) #(ML_FO (mlfo_maybe d0.inst_type #(ML_INST d0.cinst_type))) pi;
+    strengthen = (fun (ctx:(d1.cmlifyable.matype -> IIOpi (maybe d0.inst_type) pi)) -> 
+      (fun (f:(x:fin -> IIO fout (fpre x) (fpost x))) -> 
+        (** TODO: import the result **)
+        (let ctx' = strengthen_out d1.cmlifyable.matype _ #d0 pi ctx in 
+        enforce_post pi (fun x -> cpre) (fun x -> cpost) #d2 ctx' (d1.cmlifyable.mlify f)) <: IIO (maybe cout) cpre cpost))
   }
